dijkstra/verif_dijkstra3.v
@@ -7,13 +7,9 @@ Require Import CertiGraph.dijkstra.dijkstra_constants.
 
 Local Open Scope Z_scope.
 
-Section DijkstraProof.
-
   (* The invariants have been dragged out of the
      proof for readability and reuse
    *)
-
-  Context {Z_EqDec : EquivDec.EqDec Z eq}.
 
   Definition src_picked_first h src (popped: list V) :=
     0 < Zlength (heap_items h) ->
@@ -984,7 +980,7 @@ Section DijkstraProof.
             clear Htemp.
             destruct (H1 _ H_u_valid) as [_ [_ ?]].
 
-            clear -Hconn Hequ H18 H16 H15 H10 H6 H4 H_u_valid Hz Hd H1 H10' H12 Hd' Ha Ht Z_EqDec.
+            clear -Hconn Hequ H18 H16 H15 H10 H6 H4 H_u_valid Hz Hd H1 H10' H12 Hd' Ha Ht.
 
             assert (Hai: v :: popped <> []) by inversion 1.
             specialize (H4 Hai). clear Hai.
@@ -1992,7 +1988,7 @@ Section DijkstraProof.
             pose proof (Zlength_nonneg (heap_items hc)).
             lia.
           }
-            clear -H29 Hac Hab Hz Z_EqDec.
+            clear -H29 Hac Hab Hz.
           assert (forall v, vvalid g v <-> In v popped). {
             intros. split; intros.
             - destruct (In_dec Z_EqDec v popped); trivial.
@@ -2102,5 +2098,3 @@ Section DijkstraProof.
     rewrite (SpaceAdjMatGraph_unfold _ id _ _ addresses u); trivial.
     entailer!.
   Qed.
-
-End DijkstraProof.
