prim/prim_env.v
@@ -6,3 +6,5 @@ Require Export CertiGraph.lib.find_lemmas.
 Require Export CertiGraph.graph.graph_model.
 Require Export CertiGraph.graph.graph_gen.
 Require Export CertiGraph.graph.graph_relation.
+
+#[export] Instance Z_EqDec : EquivDec.EqDec Z eq := Z.eq_dec.
