priq/verif_priq_arr.v
@@ -8,13 +8,12 @@ Section PQProof.
 
 Context {size : Z}.
 Context {inf : Z}.
-Context {Z_EqDec : EquivDec.EqDec Z eq}. 
 
 #[local] Instance CompSpecs : compspecs. Proof. make_compspecs prog. Defined.
 Definition Vprog : varspecs. mk_varspecs prog. Defined.
 Local Open Scope Z_scope.
 
-Lemma body_init: semax_body Vprog (@Gprog size inf _ _) f_init (@init_spec size _). 
+Lemma body_init: semax_body Vprog (@Gprog size inf _) f_init (@init_spec size _). 
 Proof.
   start_function.
   assert (Int.max_signed < Int.max_unsigned) by now compute.
@@ -27,10 +26,10 @@ Proof.
   apply derives_refl.
 Qed.
 
-Lemma body_push: semax_body Vprog (@Gprog size inf _ _) f_push (@push_spec size inf _). 
+Lemma body_push: semax_body Vprog (@Gprog size inf _) f_push (@push_spec size inf _). 
 Proof. start_function. forward. entailer!. Qed.
 
-Lemma body_pq_emp: semax_body Vprog (@Gprog size inf _ _) f_pq_emp (@pq_emp_spec size inf _).
+Lemma body_pq_emp: semax_body Vprog (@Gprog size inf _) f_pq_emp (@pq_emp_spec size inf _).
 Proof.
   start_function.
   forward_for_simple_bound
@@ -66,10 +65,10 @@ Proof.
     symmetry; trivial.
 Qed.
 
-Lemma body_adjustWeight: semax_body Vprog (@Gprog size inf _ _) f_adjustWeight (@adjustWeight_spec size inf _).
+Lemma body_adjustWeight: semax_body Vprog (@Gprog size inf _) f_adjustWeight (@adjustWeight_spec size inf _).
 Proof. start_function. forward. entailer!. Qed.
 
-Lemma body_popMin: semax_body Vprog (@Gprog size inf _ _) f_popMin (@popMin_spec size inf _ _).
+Lemma body_popMin: semax_body Vprog (@Gprog size inf _) f_popMin (@popMin_spec size inf _).
 Proof.
   start_function.
   assert_PROP (Zlength priq_contents = size). {
